src/SMT_terms.v
@@ -1323,9 +1323,9 @@ Module Atom.
    | UO_Zneg
    | UO_Zopp
    | UO_BVbitOf (_: N) (_: nat)
-   | UO_BVnot (_: N)
-   | UO_BVneg (_: N).
-
+   | UO_BVnot   (_: N)
+   | UO_BVneg   (_: N)
+   | UO_BVextr  (n: N) (i: N) (j: N) (H0: (n >= j)%N) (H1: (j >= i)%N).
 
   Inductive binop : Type :=
    | BO_Zplus
@@ -1387,6 +1387,7 @@ Module Atom.
    | UO_BVbitOf s1 n, UO_BVbitOf s2 m => Nat_eqb n m && N.eqb s1 s2
    | UO_BVnot s1, UO_BVnot s2 => N.eqb s1 s2
    | UO_BVneg s1, UO_BVneg s2 => N.eqb s1 s2
+   | UO_BVextr s1 i1 j1 _ _, UO_BVextr s2 i2 j2 _ _ => N.eqb s1 s2 && N.eqb i1 i2 && N.eqb j1 j2
    | _,_ => false
    end.
 
@@ -1455,7 +1456,7 @@ Module Atom.
 
   Lemma reflect_uop_eqb : forall o1 o2, reflect (o1 = o2) (uop_eqb o1 o2).
   Proof.
-    intros [ | | | | | s1 n1 | s1 | s1 ] [ | | | | |s2 n2 | s2 | s2];simpl; try constructor;trivial; try discriminate.
+    intros [ | | | | | s1 n1 | s1 | s1 | s1 ] [ | | | | |s2 n2 | s2 | s2 |s2 ];simpl; try constructor;trivial; try discriminate.
     - apply iff_reflect. case_eq (Nat_eqb n1 n2).
       + case_eq ((s1 =? s2)%N).
         * rewrite N.eqb_eq, beq_nat_true_iff.
@@ -1473,6 +1474,17 @@ Module Atom.
     - apply iff_reflect. rewrite N.eqb_eq. split; intro H.
       + now inversion H.
       + now rewrite H.
+    - intros. apply iff_reflect. split. intro H.
+      inversion H.
+      rewrite !andb_true_iff; split.
+      split; now rewrite N.eqb_eq.
+      now rewrite N.eqb_eq.
+      intros. rewrite !andb_true_iff in H.
+      destruct H as ((Ha, Hb), Hc).
+      rewrite N.eqb_eq in Ha, Hb, Hc.
+      subst.
+      rewrite (proof_irrelevance H0 H2).
+      rewrite (proof_irrelevance H1 H3). reflexivity.
   Qed.
 
 
@@ -1619,6 +1631,7 @@ Qed.
         | UO_BVbitOf s _ => (Typ.TBV s, Typ.Tbool)
         | UO_BVnot s => (Typ.TBV s, Typ.TBV s)
         | UO_BVneg s => (Typ.TBV s, Typ.TBV s)
+        | UO_BVextr s i j H0 H1 => (Typ.TBV s, Typ.TBV (j - i))
         end.
 
       Definition typ_bop o := 
@@ -1795,7 +1808,15 @@ Qed.
 
          (case (Typ.eqb (get_type h) (Typ.TBV n))).
            left. exists (Typ.TBV n). now rewrite N.eqb_refl; easy.
-           right. intros. rewrite andb_false_r. easy.        
+           right. intros. rewrite andb_false_r. easy. 
+           
+         (case (Typ.eqb (get_type h) (Typ.TBV n))).
+           left. exists (Typ.TBV (j - i)). now rewrite N.eqb_refl; easy.
+           right. intros. rewrite andb_false_r. easy. 
+           
+         (case (Typ.eqb (get_type h) (Typ.TBV n))).
+           left. exists (Typ.TBV (j - i)). now rewrite N.eqb_refl; easy.
+           right. intros. rewrite andb_false_r. easy. 
         
 
         (* Binary operators *)
@@ -1989,8 +2010,6 @@ Qed.
         | CO_BV bv s => Bval (Typ.TBV s) (BITVECTOR_LIST._of_bits bv s)
         end.
 
-
-
       Definition interp_uop o :=
         match o with
         | UO_xO   => apply_unop Typ.Tpositive Typ.Tpositive xO
@@ -2001,8 +2020,9 @@ Qed.
         | UO_BVbitOf s n => apply_unop (Typ.TBV s) Typ.Tbool (BITVECTOR_LIST.bitOf n)
         | UO_BVnot s => apply_unop (Typ.TBV s) (Typ.TBV s) (@BITVECTOR_LIST.bv_not s)
         | UO_BVneg s => apply_unop (Typ.TBV s) (Typ.TBV s) (@BITVECTOR_LIST.bv_neg s)
+        | UO_BVextr s i j H0 H1 => 
+          apply_unop (Typ.TBV s) (Typ.TBV (j - i)) (@BITVECTOR_LIST.bv_extr s i j H0 H1)
         end.
-
 
 
       Definition interp_bop o :=
@@ -2200,8 +2220,11 @@ Qed.
         exists 0%Z; auto.
         exists (BITVECTOR_LIST._of_bits l n0). unfold is_true in H. rewrite N.eqb_eq in H. now rewrite H.
         (* Unary operators *)
-        destruct op; intros [ | i| | | | ]; simpl; try discriminate; try rewrite Typ.eqb_spec; intro H1; destruct (check_aux_interp_hatom h) 
-        as [x Hx]; rewrite Hx; simpl; generalize x Hx; try rewrite H1; intros y Hy; try rewrite Typ.cast_refl.
+        destruct op; intros [ | ind| | | | ]; 
+        simpl; try discriminate; try rewrite Typ.eqb_spec; 
+        intros H1a; destruct (check_aux_interp_hatom h) 
+        as [x Hx]; rewrite Hx; simpl; generalize x Hx; 
+        try rewrite H1a; intros y Hy; try rewrite Typ.cast_refl.
         exists (y~0)%positive; auto.
         exists (y~1)%positive; auto.
         exists (Zpos y); auto.
@@ -2228,6 +2251,18 @@ Qed.
         revert x y Hx Hy.
         rewrite Hb. intros.
         exists (@BITVECTOR_LIST.bv_neg n y); auto. rewrite Typ.cast_refl; auto.
+        (* bv_extr *)
+        intros.
+        apply andb_true_iff in H. destruct H as (Ha, Hb).
+        rewrite N.eqb_eq in Ha.
+        revert x y Hx Hy Hb.
+        rewrite <- Ha in *. intros.
+        apply Typ.eqb_spec in Hb.
+        revert x y Hx Hy.
+        rewrite Hb. intros.
+        exists (@BITVECTOR_LIST.bv_extr n i j H0 H1 y); auto. rewrite Typ.cast_refl; auto.
+        
+
   (* Binary operators *)
         destruct op as [ | | | | | | | A |s1|s2| s3 | s4 | s5 | s6 | s7 | s8 | n m | ti te | ti te];
           [ intros [ ti' te' | i | | | |s ] |
@@ -2501,7 +2536,12 @@ Qed.
             specialize (H (Typ.TBV n)). simpl in H. rewrite andb_false_iff in H.
             destruct H as [ H | H].
               rewrite N.eqb_refl in H. now contradict H.
-              now rewrite H.              
+              now rewrite H.
+            (* bv_extr *)
+            specialize (H (Typ.TBV (j - i))). simpl in H. rewrite andb_false_iff in H.
+            destruct H as [ H | H].
+              rewrite N.eqb_refl in H. now contradict H.
+              now rewrite H.             
         (* Binary operators *)
         destruct op; simpl; intro H; destruct (check_aux_interp_hatom h1) as [v1 Hv1]; 
         destruct (check_aux_interp_hatom h2) as [v2 Hv2]; rewrite Hv1, Hv2; simpl;
@@ -2806,7 +2846,7 @@ Qed.
         exists 0%Z; auto.
         exists (BITVECTOR_LIST._of_bits l n); auto.
         (* Unary operators *)
-        intros [ | | | | | | | ] i H; simpl; destruct (IH i H) as [x Hx]; rewrite Hx; simpl.
+        intros [ | | | | | | | | ] i H; simpl; destruct (IH i H) as [x Hx]; rewrite Hx; simpl.
         case (Typ.cast (v_type Typ.type interp_t (a .[ i])) Typ.Tpositive); simpl; try (exists true; auto); intro k; exists ((k interp_t x)~0)%positive; auto.
         case (Typ.cast (v_type Typ.type interp_t (a .[ i])) Typ.Tpositive); simpl; try (exists true; auto); intro k; exists ((k interp_t x)~1)%positive; auto.
         case (Typ.cast (v_type Typ.type interp_t (a .[ i])) Typ.Tpositive); simpl; try (exists true; auto); intro k; exists (Zpos (k interp_t x)); auto.
@@ -2815,6 +2855,8 @@ Qed.
         case (Typ.cast (v_type Typ.type interp_t (a .[ i])) (Typ.TBV n)); simpl; [ | exists true; auto]. intro k; exists (BITVECTOR_LIST.bitOf n0 (k interp_t x)) ; auto.
         case (Typ.cast (v_type Typ.type interp_t (a .[ i])) (Typ.TBV n)); simpl; [ | exists true; auto]. intro k; exists (BITVECTOR_LIST.bv_not (k interp_t x)) ; auto.
         case (Typ.cast (v_type Typ.type interp_t (a .[ i])) (Typ.TBV n)); simpl; [ | exists true; auto]. intro k; exists (BITVECTOR_LIST.bv_neg (k interp_t x)) ; auto.
+        case (Typ.cast (v_type Typ.type interp_t (a .[ i])) (Typ.TBV n)); 
+        simpl; [ | exists true; auto]. intro k; exists (BITVECTOR_LIST.bv_extr H0 H1 (k interp_t x)) ; auto.
 
        (* Binary operators *)
         intros [ | | | | | | |A | | | | | | | | | | ti te| ti te] h1 h2; simpl; rewrite andb_true_iff; intros [H1 H2]; destruct (IH h1 H1) as [x Hx]; destruct (IH h2 H2) as [y Hy]; rewrite Hx, Hy; simpl.
@@ -2995,9 +3037,6 @@ Qed.
   Qed.
 
 End Atom.
-
-
-
 
 Arguments Atom.Val {_} {_} _ _.
 
